\begin{frame}
  \frametitle{Strassen's Algorithm}
  \centering
  \large
\onslide<1->{
  $
  \mathbf{A B = C}
  $
}

\onslide<2->{


\medskip
  $
  \begin{bmatrix}
  A_{11} & A_{12}\\
  A_{21} & A_{22}
  \end{bmatrix}
  \begin{bmatrix}
  B_{11} & B_{12}\\
  B_{21} & B_{22}
  \end{bmatrix}
  =
  \begin{bmatrix}
  C_{11} & C_{12}\\
  C_{21} & C_{22}
  \end{bmatrix}
  $
  }


  \onslide<3->{

\medskip
$
C_{11} = A_{11} \cdot B_{11} + A_{12} \cdot B_{21}
$

$
C_{12} = A_{11} \cdot B_{12} + A_{12} \cdot B_{22}
$

$
C_{21} = A_{21} \cdot B_{11} + A_{22} \cdot B_{21}
$

$
C_{22} = A_{21} \cdot B_{12} + A_{22} \cdot B_{22}
$
}
\end{frame}

\input{slides/algo.tex}

\input{slides/BigO.tex}


\begin{frame}
  \frametitle{Strassen's Algorithm}
  \begin{columns}
    \begin{column}{0.5\textwidth}
      \onslide<1->{
      \large
      \begin{math}
      \begin{aligned}
      \text{I}   &= (A_{11} + A_{22}) \cdot (B_{11} + B_{22}) \\
      \text{II}  &= (A_{21} + A_{22}) \cdot B_{11} \\
      \text{III} &= A_{11} \cdot (B_{12}-B_{22}) \\
      \text{IV}  &= A_{22} \cdot (-B_{11}+B_{21}) \\
      \text{V}   &= (A_{11} + A_{12}) \cdot B_{22} \\
      \text{VI}  &= (-A_{11} + A_{21}) \cdot (B_{11} + B_{12}) \\
      \text{VII} &= (A_{12} - A_{22}) \cdot (B_{21} + B_{22}) \\
      \end{aligned}
      \end{math}
      }
    \end{column}

    \begin{column}{0.5\textwidth}
        \onslide<2->{
        \large
        \begin{math}
        \begin{aligned}
        C_{11} &= \text{I} + \text{IV} - \text{V} + \text{VII} \\
        C_{21} &= \text{II} + \text{IV} \\
        C_{12} &= \text{III} + \text{V}\\
        C_{22} &= \text{I} + \text{III} - \text{II} + \text{VI} \\
        \end{aligned}
        \end{math}
        }
    \end{column}
\end{columns}

\onslide<3->{

\bigskip
\centering
\tiny
\begin{math}
\begin{aligned}
  C_{11} &= (A_{11} + A_{22}) \cdot (B_{11} + B_{22}) + A_{22} \cdot (-B_{11}+B_{21}) - (A_{11} + A_{12}) \cdot B_{22} + (A_{12} - A_{22}) \cdot (B_{21} + B_{22}) \\
  C_{11} &= A_{11}B_{11} + A_{11}B_{22} + A_{22}B_{11} + A_{22}B_{22} -A_{22}B_{11}+A_{22}B_{21} - A_{11}B_{22} - A_{12}B_{22}+ A_{12}B_{21} + A_{12}B_{22} - A_{22}B_{21} - A_{22}B_{22} \\
  C_{11} &= A_{11}B_{11} + A_{12}B_{21}
\end{aligned}
\end{math}
}

\end{frame}


\begin{frame}
\begin{adjustbox}{width=\textwidth}
\begin{tikzpicture}[ampersand replacement=\&]

  \foreach \i in {1,...,4}
  {
  \small{
    \matrix (X\i)[matrix of math nodes,nodes in empty cells,
              nodes = {draw, minimum size=10mm,
                       anchor=center,
                       inner sep=0pt, outer sep=0pt},
              column sep=-\pgflinewidth,
              row sep=-\pgflinewidth,
              ] at (0,-\i*5)
   {
   A_{11}B_{11} \& A_{12}B_{11} \& A_{21}B_{11} \& A_{22}B_{11} \\
   A_{11}B_{21} \& A_{12}B_{21} \& A_{21}B_{21} \& A_{22}B_{21} \\
   A_{11}B_{11} \& A_{12}B_{12} \& A_{21}B_{12} \& A_{22}B_{12} \\
   A_{11}B_{22} \& A_{12}B_{22} \& A_{21}B_{22} \& A_{22}B_{22} \\
   };}

    \foreach \j in {1,...,7}
    {
    \matrix(M\i\j)[matrix of math nodes,nodes in empty cells,
                nodes = {draw, minimum size=10mm,
                         anchor=center,
                         inner sep=0pt, outer sep=0pt},
                column sep=-\pgflinewidth,
                row sep=-\pgflinewidth,
                ] at (\j*5,-\i*5)
     {
     \& \& \& \\
     \& \& \& \\
     \& \& \& \\
     \& \& \& \\
     };
   }
 }

\huge{
 \node at (-3,-20)  {$C_{22}=$};
 \node at (-3,-15) {$C_{21}=$} ;
 \node at (-3,-10) {$C_{12}=$} ;
 \node at (-3,-5) {$C_{11}=$} ;

 \node at (5,-2)  {I};
 \node at (10,-2)  {II};
 \node at (15,-2)  {III};
 \node at (20,-2)  {IV};
 \node at (25,-2)  {V};
 \node at (30,-2)  {VI};
 \node at (35,-2)  {VII};
 }


 \node[opacity=0.5, rounded corners=0pt, inner sep=-1pt, fill=green, fit=(X1-1-1)] {};
 \node[opacity=0.5, rounded corners=0pt, inner sep=-1pt, fill=green, fit=(X1-2-2)] {};
 \node[opacity=0.5, rounded corners=0pt, inner sep=-1pt, fill=green, fit=(X2-3-1)] {};
 \node[opacity=0.5, rounded corners=0pt, inner sep=-1pt, fill=green, fit=(X2-4-2)] {};
 \node[opacity=0.5, rounded corners=0pt, inner sep=-1pt, fill=green, fit=(X3-1-3)] {};
 \node[opacity=0.5, rounded corners=0pt, inner sep=-1pt, fill=green, fit=(X3-2-4)] {};
 \node[opacity=0.5, rounded corners=0pt, inner sep=-1pt, fill=green, fit=(X4-3-3)] {};
 \node[opacity=0.5, rounded corners=0pt, inner sep=-1pt, fill=green, fit=(X4-4-4)] {};

 \node[opacity=0.5, rounded corners=0pt, inner sep=-1pt, fill=green, fit=(M11-4-1)] {};
 \node[opacity=0.5, rounded corners=0pt, inner sep=-1pt, fill=green, fit=(M11-1-4)] {};
 \node[opacity=0.5, rounded corners=0pt, inner sep=-1pt, fill=green, fit=(M11-4-4)] {};
 \node[opacity=0.5, rounded corners=0pt, inner sep=-1pt, fill=green, fit=(M11-1-1)] {};
 \node[opacity=0.5, rounded corners=0pt, inner sep=-1pt, fill=red, fit=(M14-1-4)] {};
 \node[opacity=0.5, rounded corners=0pt, inner sep=-1pt, fill=green, fit=(M14-2-4)] {};
 \node[opacity=0.5, rounded corners=0pt, inner sep=-1pt, fill=red, fit=(M15-4-1)] {};
 \node[opacity=0.5, rounded corners=0pt, inner sep=-1pt, fill=red, fit=(M15-4-2)] {};
 \node[opacity=0.5, rounded corners=0pt, inner sep=-1pt, fill=red, fit=(M17-2-4)] {};
 \node[opacity=0.5, rounded corners=0pt, inner sep=-1pt, fill=red, fit=(M17-4-4)] {};
 \node[opacity=0.5, rounded corners=0pt, inner sep=-1pt, fill=green, fit=(M17-2-2)] {};
 \node[opacity=0.5, rounded corners=0pt, inner sep=-1pt, fill=green, fit=(M17-4-2)] {};

 \node[opacity=0.5, rounded corners=0pt, inner sep=-1pt, fill=green, fit=(M23-3-1)] {};
 \node[opacity=0.5, rounded corners=0pt, inner sep=-1pt, fill=red, fit=(M23-4-1)] {};
 \node[opacity=0.5, rounded corners=0pt, inner sep=-1pt, fill=green, fit=(M25-4-1)] {};
 \node[opacity=0.5, rounded corners=0pt, inner sep=-1pt, fill=green, fit=(M25-4-2)] {};

 \node[opacity=0.5, rounded corners=0pt, inner sep=-1pt, fill=green, fit=(M32-1-4)] {};
 \node[opacity=0.5, rounded corners=0pt, inner sep=-1pt, fill=green, fit=(M32-1-3)] {};
 \node[opacity=0.5, rounded corners=0pt, inner sep=-1pt, fill=red, fit=(M34-1-4)] {};
 \node[opacity=0.5, rounded corners=0pt, inner sep=-1pt, fill=green, fit=(M34-2-4)] {};

 \node[opacity=0.5, rounded corners=0pt, inner sep=-1pt, fill=green, fit=(M41-4-1)] {};
 \node[opacity=0.5, rounded corners=0pt, inner sep=-1pt, fill=green, fit=(M41-1-4)] {};
 \node[opacity=0.5, rounded corners=0pt, inner sep=-1pt, fill=green, fit=(M41-4-4)] {};
 \node[opacity=0.5, rounded corners=0pt, inner sep=-1pt, fill=green, fit=(M41-1-1)] {};
 \node[opacity=0.5, rounded corners=0pt, inner sep=-1pt, fill=red, fit=(M42-1-4)] {};
 \node[opacity=0.5, rounded corners=0pt, inner sep=-1pt, fill=red, fit=(M42-1-3)] {};
 \node[opacity=0.5, rounded corners=0pt, inner sep=-1pt, fill=green, fit=(M43-3-1)] {};
 \node[opacity=0.5, rounded corners=0pt, inner sep=-1pt, fill=red, fit=(M43-4-1)] {};
 \node[opacity=0.5, rounded corners=0pt, inner sep=-1pt, fill=green, fit=(M46-1-3)] {};
 \node[opacity=0.5, rounded corners=0pt, inner sep=-1pt, fill=red, fit=(M46-1-1)] {};
 \node[opacity=0.5, rounded corners=0pt, inner sep=-1pt, fill=green, fit=(M46-3-3)] {};
 \node[opacity=0.5, rounded corners=0pt, inner sep=-1pt, fill=red, fit=(M46-3-1)] {};
\end{tikzpicture}
\end{adjustbox}
\end{frame}


\begin{frame}
  \frametitle{Strassen's Algorithm}
  \begin{columns}
    \begin{column}{0.5\textwidth}
      \large
      \begin{math}
      \begin{aligned}
      \text{I}   &= (A_{11} + A_{22}) \cdot (B_{11} + B_{22}) \\
      \text{II}  &= (A_{21} + A_{22}) \cdot B_{11} \\
      \text{III} &= A_{11} \cdot (B_{12}-B_{22}) \\
      \text{IV}  &= A_{22} \cdot (-B_{11}+B_{21}) \\
      \text{V}   &= (A_{11} + A_{12}) \cdot B_{22} \\
      \text{VI}  &= (-A_{11} + A_{21}) \cdot (B_{11} + B_{12}) \\
      \text{VII} &= (A_{12} - A_{22}) \cdot (B_{21} + B_{22}) \\
      \end{aligned}
      \end{math}

    \end{column}

    \begin{column}{0.5\textwidth}
        \large
        \begin{math}
        \begin{aligned}
        C_{11} &= \text{I} + \text{IV} - \text{V} + \text{VII} \\
        C_{21} &= \text{II} + \text{IV} \\
        C_{12} &= \text{III} + \text{V}\\
        C_{22} &= \text{I} + \text{III} - \text{II} + \text{VI} \\
        \end{aligned}
        \end{math}

    \end{column}
\end{columns}
\end{frame}



\begin{frame}

\begin{columns}
  \begin{column}{0.5\textwidth}
\large
\begin{math}
\begin{aligned}
\text{\textbf{I}}   &= (\mathbf{A_{11}} + \mathbf{A_{22}}) \cdot (\mathbf{B_{11}} + \mathbf{B_{22}}) \\
\text{\textbf{II}}  &= (\mathbf{A_{21}} + \mathbf{A_{22}}) \cdot \mathbf{B_{11}} \\
\text{\textbf{III}} &= \mathbf{A_{11}} \cdot (\mathbf{B_{12}}-\mathbf{B_{22}}) \\
\text{\textbf{IV}}  &= \mathbf{A_{22}} \cdot (-\mathbf{B_{11}}+\mathbf{B_{21}}) \\
\text{\textbf{V}}   &= (\mathbf{A_{11}} + \mathbf{A_{12}}) \cdot \mathbf{B_{22}} \\
\text{\textbf{VI}}  &= (-\mathbf{A_{11}} + \mathbf{A_{21}}) \cdot (\mathbf{B_{11}} + \mathbf{B_{12}}) \\
\text{\textbf{VII}} &= (\mathbf{A_{12}} - \mathbf{A_{22}}) \cdot (\mathbf{B_{21}} + \mathbf{B_{22}}) \\
\end{aligned}
\end{math}

\end{column}

\begin{column}{0.5\textwidth}
  \large
  \begin{math}
  \begin{aligned}
  \mathbf{C_{11}} &= \text{\textbf{I}} + \text{\textbf{IV}} - \text{\textbf{V}} + \text{\textbf{VII}} \\
  \mathbf{C_{21}} &= \text{\textbf{II}} + \text{\textbf{IV}} \\
  \mathbf{C_{12}} &= \text{\textbf{III}} + \text{\textbf{V}}\\
  \mathbf{C_{22}} &= \text{\textbf{I}} + \text{\textbf{III}} - \text{\textbf{II}} + \text{\textbf{VI}} \\
  \end{aligned}
  \end{math}

\end{column}
\end{columns}

\end{frame}

\begin{frame}
  \frametitle{Algorithm}
  \scalebox{0.5}{\parbox{\linewidth}{
    \begin{algorithm}[H]\caption{Strassen Matrix Multiplication}
      \setlength{\lineskip}{7pt}
      \begin{algorithmic}[1]
        \Function{MM}{$\textbf{A}, \textbf{B}, \textbf{C}, n$}
        \If{$n = 2$}
        \State  $C \gets zeros((n, n))$
        \State $P  \gets (A[0][0]+A[1][1])\cdot( B[0][0]+B[1][1])$
        \State   $Q  \gets (A[1][0]+A[1][1])\cdot B[0][0]$
        \State   $R  \gets A[0][0]\cdot (B[0][1]-B[1][1])$
        \State   $S  \gets A[1][1]\cdot (B[1][0]-B[0][0])$
        \State   $T  \gets (A[0][0]+A[0][1])\cdot B[1][1]$
        \State   $U  \gets (A[1][0]-A[0][0])\cdot (B[0][0]+B[0][1])$
        \State   $V  \gets (A[0][1]-A[1][1])\cdot (B[1][0]+B[1][1])$
        \State   $C[0][0]  \gets P+S-T+V$
        \State   $C[0][1]  \gets R+T$
        \State   $C[1][0]  \gets Q+S$
        \State   $C[1][1]  \gets P+R-Q+U$
        \Else
      \State  $ m \gets n/2$
  \State $A11, A12, A21, A22 \gets A[:m][:m], A[:m][m:], A[m:][:m], A[m:][m:]$
  \State $B11, B12, B21, B22 \gets B[:m][:m], B[:m][m:], B[m:][:m], B[m:][m:]$
  \State $C11 \gets strassen(A11, B11, m) + strassen(A12, B21, m)$
  \State $C12 \gets strassen(A11, B12, m) + strassen(A12, B22, m)$
  \State $C21 \gets strassen(A21, B11, m) + strassen(A22, B21, m)$
  \State $C22 \gets strassen(A21, B12, m) + strassen(A22, B22, m)$
  \State $  C \gets vstack((hstack((C11, C12)), hstack((C21, C22))))$

        \EndIf
        \State \textbf{return} $\textbf{C}$

       \EndFunction
      \end{algorithmic}
  \end{algorithm}
    }}
\end{frame}
